platform/cito/SetArrow.v
@@ -4,27 +4,27 @@ Require Import Equalities.
 
 Set Implicit Arguments.
 
-Module SetArrow (Key : MiniDecidableType) <: MembershipDecidableSet Key.
+Module Make (Key : MiniDecidableType) <: MembershipDecidableSet Key.
 
-  Definition set := Key.t -> bool.
+  Definition t := Key.t -> bool.
 
-  Definition mem x (s : set) := s x = true.
+  Definition mem x (s : t) := s x = true.
 
-  Definition union (a b : set) := fun x => orb (a x) (b x).
+  Definition union (a b : t) := fun x => orb (a x) (b x).
 
-  Lemma union_correct : forall a b x, mem x (union a b) <-> mem x a \/ mem x b.
+  Lemma union_spec : forall a b x, mem x (union a b) <-> mem x a \/ mem x b.
     unfold mem, union; intuition; eapply Bool.orb_true_elim in H; destruct H; intuition.
   Qed.
 
-  Definition diff (a b : set) := fun x => andb (a x) (negb (b x)).
+  Definition diff (a b : t) := fun x => andb (a x) (negb (b x)).
 
-  Lemma diff_correct : forall a b x, mem x (diff a b) <-> mem x a /\ ~ mem x b.
+  Lemma diff_spec : forall a b x, mem x (diff a b) <-> mem x a /\ ~ mem x b.
     unfold mem, diff; intuition; eapply Bool.andb_true_iff in H; destruct H; intuition; rewrite H0 in H1; intuition.
   Qed.
 
-  Definition empty : set := fun _ => false.
+  Definition empty : t := fun _ => false.
 
-  Lemma empty_correct : forall x, ~ mem x empty.
+  Lemma empty_spec : forall x, ~ mem x empty.
     unfold empty, mem; eauto.
   Qed.
 
@@ -35,7 +35,7 @@ Module SetArrow (Key : MiniDecidableType) <: MembershipDecidableSet Key.
       else
         false.
 
-  Lemma singleton_correct : forall x x', mem x' (singleton x) <-> x' = x.
+  Lemma singleton_spec : forall x x', mem x' (singleton x) <-> x' = x.
     unfold mem, singleton; intros; destruct (Key.eq_dec x' x); intuition; intuition; discriminate.
   Qed.
 
@@ -47,4 +47,4 @@ Module SetArrow (Key : MiniDecidableType) <: MembershipDecidableSet Key.
   Include Relations Key.
   Include Util Key.
 
-End SetArrow.
+End Make.
