platform/cito/TempVars.v
@@ -1,0 +1,9 @@
+Require Import TempVarsList.
+Require Import StringSet.
+Require Import SetUtil.
+
+Set Implicit Arguments.
+
+Definition make_temp_vars_range start len := to_set (make_temp_vars_range_list start len).
+
+Definition make_temp_vars := make_temp_vars_range 0.
