platform/cito/TempVarsList.v
@@ -1,0 +1,7 @@
+Require Import ReservedNames.
+
+Set Implicit Arguments.
+
+Definition make_temp_vars_range_list start len := List.map temp_var (List.seq start len).
+
+Definition make_temp_vars_list := make_temp_vars_range_list 0.
